Soundness.v
@@ -6,9 +6,9 @@ From Elo Require Import Array.
 From Elo Require Import Map.
 From Elo Require Import Core.
 From Elo Require Import Access.
-From Elo Require Import WBA.
+From Elo Require Import References.
 
-Lemma context_weakening : forall Gamma Gamma' t T,
+Local Lemma context_weakening : forall Gamma Gamma' t T,
   Gamma' |-- t is T ->
   Gamma includes Gamma' ->
   Gamma  |-- t is T.
@@ -18,7 +18,7 @@ Proof.
   eauto using well_typed_term, update_preserves_inclusion.
 Qed.
 
-Lemma context_weakening_empty : forall Gamma t T,
+Local Lemma context_weakening_empty : forall Gamma t T,
   empty |-- t is T ->
   Gamma |-- t is T.
 Proof.
@@ -26,27 +26,10 @@ Proof.
 Qed.
 
 (* ------------------------------------------------------------------------- *)
-(* TODO                                                                      *)
-(* ------------------------------------------------------------------------- *)
-
-Lemma deterministic_typing : forall Gamma t T1 T2,
-  Gamma |-- t is T1 ->
-  Gamma |-- t is T2 ->
-  T1 = T2.
-Proof.
-Admitted.
-
-Ltac apply_deterministic_typing :=
-  match goal with
-  | H1 : _ |-- ?t is ?T1, H2 : _ |-- ?t is ?T2 |- _ =>
-    assert (T1 = T2) by eauto using deterministic_typing; subst
-  end.
-
-(* ------------------------------------------------------------------------- *)
 (* preservation                                                              *)
 (* ------------------------------------------------------------------------- *)
 
-Lemma preservation_subst : forall t tx T Tx Tx' Gamma x,
+Local Lemma preservation_subst : forall t tx T Tx Tx' Gamma x,
   Gamma |-- (TM_Fun x Tx t) is (TY_Fun Tx' T) ->
   empty |-- tx is Tx' ->
   Gamma |-- [x := tx] t is T.
@@ -63,7 +46,7 @@ Proof.
     eauto using well_typed_term, context_weakening, context_weakening_empty,
       update_overwrite, update_permutation.
   }
-  intros * ?. inversion_type. intros. eapply H; eauto.
+  intros * ?. inversion_type. intros. eauto.
 Qed.
 
 Theorem preservation : forall m m' t t' eff T,
@@ -72,29 +55,14 @@ Theorem preservation : forall m m' t t' eff T,
   m / t ==[eff]==> m' / t' ->
   empty |-- t' is T.
 Proof.
-  intros * Hwtr Htype ?. inversion_mstep; generalize dependent t'.
-  remember empty as Gamma.
-  - clear Hwtr.
-    induction Htype; intros; inversion_step;
-    eauto using well_typed_term, preservation_subst.
-  - clear Hwtr.
-    induction Htype; intros; inversion_step;
-    eauto using well_typed_term.
-  - induction Htype; intros;
-    inversion_step; inversion_clear Hwtr; subst;
-    eauto using well_typed_term;
-    inversion Htype; subst.
-    + match goal with
-      | Hwtr' : well_typed_references _ _ |- _ =>
-        inversion Hwtr'; subst
-      end.
-      eauto using context_weakening_empty.
-    + match goal with
-      | Hwtr' : well_typed_references _ _ |- _ =>
-        inversion Hwtr'; subst
-      end.
-      eauto using context_weakening_empty.
-  - induction Htype; intros; inversion_step; try (inversion Hwtr; subst);
-    eauto using well_typed_term.
+  intros * Hwtr ? ?. inversion_mstep; generalize dependent t';
+  remember empty as Gamma;
+  induction_type; intros; inversion_step; inversion_clear Hwtr;
+  eauto using well_typed_term, preservation_subst;
+  inversion_type;
+  match goal with
+  | H : well_typed_references _ _ |- _ => inversion_clear H
+  end;
+  eauto using context_weakening_empty.
 Qed.
 
